LoL/MonadAlgebras/EffectObservations.lean
@@ -1,43 +1,98 @@
+import Mathlib.Order.CompleteLattice.Basic
+
 import LoL.MonadUtil
 import LoL.SpecMonad
 
 universe u v w
 
-variable (m : Type u -> Type w)
+variable (m : Type v -> Type u)
 
+class MProp [Monad m] (l : outParam (Type v)) where
+  μ : m l -> l
+  pure : ∀ l, μ (pure l) = l
+  bind : ∀ {α : Type v} (x : m α) (f g : α -> m l),
+    μ ∘ f = μ ∘ g ->
+    μ (x >>= f) = μ (x >>= g)
 
-class MonadAlgebra [Monad m] (l : outParam (Type u)) where
-  morphism : m l -> l
-  pure (y : l) : morphism (pure y) = y
-  bind {α : Type u} (y : m α) (f : α -> m l) : morphism (y >>= f) = (morphism $ (morphism ∘ f) <$> y)
+abbrev MProp.lift {m : Type u -> Type v} {l : Type u} [Monad m] [MProp m l] :
+  {α : Type u} -> m α -> Cont l α := fun x f => μ $ f <$> x
 
-abbrev MonadAlgebra.lift {m} {t : Type u} [Monad m] [LawfulMonad m] [MonadAlgebra m t] :
-  {α : Type u} -> m α -> Cont t α := fun x f => MonadAlgebra.morphism $ f <$> x
+instance (l : Type u) {m : Type u -> Type v} [Monad m] [MProp m l] : MonadLiftT m (Cont l) where
+  monadLift := MProp.lift
 
-instance (t : Type u) [Monad m] [LawfulMonad m] [MonadAlgebra m t] : MonadLiftT m (Cont t) where
-  monadLift := MonadAlgebra.lift
-
-instance (t : Type u) [Monad m] [LawfulMonad m] [MonadAlgebra m t] : LawfulMonadLift m (Cont t) where
+instance (l : Type u) {m : Type u -> Type v} [Monad m] [LawfulMonad m] [MProp m l] : LawfulMonadLift m (Cont l) where
   lift_pure := by
-    intro α x; unfold monadLift instMonadLiftTContOfLawfulMonadOfMonadAlgebra;
-    simp; unfold MonadAlgebra.lift; simp [monadLift, pure, map_pure, MonadAlgebra.pure]
+    intro α x; simp [monadLift, pure]; unfold MProp.lift; simp [map_pure, MProp.pure]
   lift_bind := by
-    intros α β x f; unfold monadLift instMonadLiftTContOfLawfulMonadOfMonadAlgebra;
-    simp; unfold MonadAlgebra.lift; ext g; simp [monadLift, bind, MonadAlgebra.bind]; rfl
+    intros α β x f; simp [monadLift, bind]; unfold MProp.lift; ext g
+    rw (config := { occs := .pos [2] }) [map_eq_pure_bind]
+    simp only [map_bind]; apply MProp.bind
+    ext; simp [MProp.pure]
 
-class MonadAlgebraOrdered [Monad m] (x : outParam (Type u)) [Preorder x] extends MonadAlgebra m x where
-  bind_le : ∀ {α : Type u} (y : m α) (f f' : α -> x),
-    (∀ a, f a ≤ f' a) → morphism (f <$> y) ≤ morphism (f' <$> y)
+class MPropOrdered (l : outParam (Type v)) [Monad m] [PartialOrder l] where
+  μ : m l -> l
+  μ_ord_pure : ∀ l, μ (pure l) = l
+  μ_ord_bind {α : Type v} :
+    ∀ (f g : α -> m l), μ ∘ f ≤ μ ∘ g ->
+      ∀ x : m α, μ (x >>= f) ≤ μ (x >>= g)
 
-lemma Cont.monotone_lift {t : Type u} [Monad m] [LawfulMonad m] [Preorder t] [MonadAlgebraOrdered m t] :
-  ∀ {α : Type u} (x : m α), MonadAlgebra.lift x |>.monotone := by
-  unfold Cont.monotone; intros; unfold MonadAlgebra.lift
-  solve_by_elim [MonadAlgebraOrdered.bind_le]
+@[reducible]
+instance OfMPropPartialOrdered {m : Type u -> Type v} {l : Type u} [Monad m] [PartialOrder l] [mprop : MPropOrdered m l] : MProp m l where
+  μ := MPropOrdered.μ
+  pure := MPropOrdered.μ_ord_pure
+  bind := by intros; apply PartialOrder.le_antisymm
+    <;> apply MPropOrdered.μ_ord_bind
+    <;> simp_all only [le_refl]
 
-def triple {l α} [Monad m] [LawfulMonad m] [Preorder l] [MonadAlgebra m l]
-  (pre : l) (c : m α) (post : α -> l) := pre ≤ liftM (n := Cont l) c post
+lemma MPropOrdered.bind {α : Type u} {m} {l : Type u} [Monad m] [PartialOrder l] [MPropOrdered m l] :
+    ∀ (x : m α) (f g : α -> m l), μ ∘ f = μ ∘ g ->
+     μ (x >>= f) = μ (x >>= g) := MProp.bind
 
--- instance (t : Type u) [MonadOrder m] [LawfulMonad m] [Preorder t] [MonadAlgebraOrdered m t] : LawfulMonadLift m (W t) where
---   monadLift := fun x => ⟨MonadAlgebra.lift x, Cont.monotone_lift m x⟩
---   monadMapPure := by intros; unfold MonadAlgebra.lift; simp [monadLift, pure, map_pure, MonadAlgebra.pure]
---   monadMapBind := by intros; ext g; simp [monadLift, bind, MonadAlgebra.bind, MonadAlgebra.lift]; rfl
+lemma Cont.monotone_lift {l : Type u} {m : Type u -> Type v} [Monad m] [LawfulMonad m] [PartialOrder l] [MPropOrdered m l] :
+  ∀ {α : Type u} (x : m α), MProp.lift x |>.monotone := by
+  unfold Cont.monotone; intros; simp [MProp.lift]; rw [map_eq_pure_bind, map_eq_pure_bind]
+  apply MPropOrdered.μ_ord_bind; intro; simp [MPropOrdered.μ_ord_pure, *]
+
+open Classical in
+noncomputable def LE.pure {l : Type u} [inst: LE l] [OrderTop l] [OrderBot l] : Prop -> l := fun p =>
+  if p then ⊤ else ⊥
+
+macro "⌜" p:term "⌝" : term => `(LE.pure $p)
+
+@[app_unexpander LE.pure] def unexpandPure : Lean.PrettyPrinter.Unexpander
+  | `($(_) $p:term) => `(⌜$p:term⌝)
+  | _ => throw ()
+
+
+lemma trueE (l : Type v) [inst: LE l] [OrderTop l] [OrderBot l] : ⌜True⌝ = (⊤ : l) := by
+  simp [LE.pure]
+
+
+
+lemma falseE (l : Type v) [inst: LE l] [OrderTop l] [OrderBot l] : ⌜False⌝ = (⊥ : l) := by
+  simp [LE.pure]
+
+open Classical in
+lemma LE.pure_imp {l : Type u} [inst: LE l] [OrderTop l] [OrderBot l]
+  (p₁ p₂ : Prop) : (p₁ -> p₂) -> ⌜p₁⌝ <= (⌜p₂⌝ : l) := by
+  simp [LE.pure]; split <;> aesop
+
+lemma LE.pure_intro {l : Type u} [inst: LE l] [OrderTop l] [OrderBot l]
+  (p : Prop) (h : l) : (⌜p⌝ <= h) = (p -> ⊤ <= h) := by
+    simp [LE.pure]; split <;> aesop
+
+@[simp]
+lemma MProp.μ_eq {m l} [Monad m] [PartialOrder l] [MPropOrdered m l] : MProp.μ (m := m) = MPropOrdered.μ (m := m) := by rfl
+
+lemma MProp.lift_bind {α β} {l : Type u} {m : Type u -> Type v} [Monad m] [LawfulMonad m] [PartialOrder l] [MPropOrdered m l]
+  (x : m α) (f g : α -> Cont l β) :
+    f <= g ->
+    (lift x >>= f) ≤ (lift x >>= g) := by
+    intro fLg h; simp [Bind.bind]
+    apply Cont.monotone_lift; intros h; apply fLg
+
+class MPropDetertministic (l : outParam (Type v)) [Monad m] [CompleteLattice l] [MPropOrdered m l] where
+  /-- 😈 -/
+  demonic {α ι : Type v} (c : m α) (p : ι -> α -> l) [Nonempty ι] : ⨅ i, MProp.lift c (p i) ≤ MProp.lift c (fun x => ⨅ i, p i x)
+  /-- 😇 -/
+  angelic {α ι : Type v} (c : m α) (p : ι -> α -> l) [Nonempty ι] : MProp.lift c (fun x => ⨆ i, p i x) ≤ ⨆ i, MProp.lift c (p i)
