LoL.lean
@@ -1,3 +1,1 @@
--- This module serves as the root of the `LoL` library.
--- Import modules here that should be built as part of the library.
-import LoL.Basic
+import LoL.MonadAlgebras.NonDetT.Basic
