LoL/MProp/Instances.lean
@@ -1,5 +1,6 @@
 import LoL.MProp.EffectObservations
 import LoL.NonDetM
+import Plausible.Gen
 
 instance : Nonempty UProp := inferInstance
 
@@ -241,6 +242,34 @@ instance MPropExceptPartDetertministic (hd : ε -> Prop)
     simp [Except.getD, MProp.μ, iInf_const]; rw [inst.μ_surjective, iSup_const]; rfl
 
 end ExeceptHandler
+
+#check List.forIn'
+
+instance (g : Type) (l : Type u) (m : Type u -> Type v)
+  [PartialOrder l]
+  [Monad m] [LawfulMonad m] 
+  [inst: MPropOrdered m l] : MPropOrdered (Plausible.RandGT g m) (ULift g -> l) := 
+  inferInstanceAs (MPropOrdered (StateT (ULift g) m) (ULift g -> l))
+
+-- instance : MPropOrdered Plausible.Gen (ULift StdGen -> Prop) where
+--   μ m g := ∀ n, MPropOrdered.μ (m n) g
+--   ι p n := MPropOrdered.ι p
+--   μ_surjective := by intro p; simp; ext; rfl 
+--   μ_top := by 
+--     intro p; simp [pure, ReaderT.pure, MPropOrdered.μ];
+--     unfold StateT.pure; 
+--     simp [pure]; intro g; simp 
+--   μ_bot := by 
+--     intro p; simp [pure, ReaderT.pure, MPropOrdered.μ];
+--     unfold StateT.pure; 
+--     simp [pure]; intro g; simp 
+--   μ_ord_pure := by 
+--     intro p₁ p₂ imp; simp [pure, ReaderT.pure, MPropOrdered.μ];
+--     unfold StateT.pure; 
+--     simp [pure]; intro g; simpa
+--   μ_ord_bind := by 
+--     intro α f g le; simp [bind, ReaderT.bind, StateT.bind]
+--     intro g; simpa
 
 namespace PartialCorrectness
 scoped instance PartialHandler {ε} : IsHandler (ε := ε) fun _ => True where
