LoL/MonadAlgebras/Functors.lean
@@ -1,9 +1,0 @@
-import LoL.Functors
-import LoL.MonadAlgebras.EffectObservations
-
-universe u v w
-
-class TransformerAlgebra (t : (Type u -> Type u) -> (Type u -> Type v)) (m : outParam (Type u -> Type u))
-  [Monad m] [inst: MonadTransformer t] where
-  hasmorphism {x : Type u} [MonadAlgebra m x] :
-    @MonadAlgebra (t m) inst.isMonad (m x)
